Set_Graphs/Graph_Algorithms/Bellman_Ford_Example.thy
@@ -1,0 +1,99 @@
+theory Bellman_Ford_Example
+  imports Bellman_Ford  "HOL-Data_Structures.RBT_Map"
+begin
+
+instantiation prod::(linorder, linorder) linorder
+begin
+
+fun less_eq_prod where
+ "less_eq_prod (x, y) (a, b) = (if x < a then True 
+                                  else if x = a then y \<le> b
+                                  else False)"
+fun less_prod where
+ "less_prod (x, y) (a, b) = (if x < a then True 
+                                  else if x = a then y < b
+                                  else False)"
+instance 
+  apply(intro Orderings.linorder.intro_of_class  class.linorder.intro
+              class.order_axioms.intro class.order.intro class.preorder.intro
+              class.linorder_axioms.intro)
+  subgoal for x y 
+    by(all \<open>cases x\<close>, all \<open>cases y\<close>)
+      (auto split: if_split simp add: less_le_not_le)
+    subgoal for x  
+    by(all \<open>cases x\<close>)
+      (auto split: if_split simp add: less_le_not_le)
+  subgoal for x y z
+    apply(all \<open>cases x\<close>, all \<open>cases y\<close>, all \<open>cases z\<close>)
+    apply(auto split: if_split simp add: less_le_not_le)
+    using order.trans by metis+
+  subgoal for x y 
+    apply(all \<open>cases x\<close>, all \<open>cases y\<close>)
+    apply(auto split: if_split simp add: less_le_not_le)
+    apply presburger
+    by (metis order_antisym_conv)
+  subgoal for x y 
+    by(all \<open>cases x\<close>, all \<open>cases y\<close>)
+      (auto split: if_split simp add: less_le_not_le)
+  done
+end
+
+
+definition "connection_empty = empty"
+definition "connection_update = update"
+definition "connection_delete = RBT_Map.delete"
+definition "connection_lookup = lookup"
+definition "connection_invar = M.invar"
+
+lemma Map_connection:"Map connection_empty connection_update connection_delete connection_lookup connection_invar"
+  using RBT_Map.M.Map_axioms     
+  by(auto simp add: connection_update_def connection_empty_def  connection_delete_def
+                    connection_lookup_def connection_invar_def)
+
+lemma bellman_ford_spec: "bellman_ford_spec connection_update connection_empty connection_lookup connection_invar connection_delete"
+  using Map_connection by(auto intro!: bellman_ford_spec.intro)
+
+global_interpretation bellford: bellman_ford_spec where connection_update=connection_update
+and connection_empty=connection_empty and connection_lookup=connection_lookup
+and connection_delete=connection_delete and connection_invar=connection_invar 
+and es= es and vs=vs and edge_costs=edge_costs
+for edge_costs es vs
+defines search_rev_path_exec = bellford.search_rev_path_exec 
+and bellman_ford_init_algo = bellford.bellman_ford_init
+and  bellman_ford_algo = bellford.bellman_ford
+and relax=bellford.relax                              
+  using bellman_ford_spec by auto
+
+definition "edges = [(0::nat, 1::nat), (0, 2), (2, 3), (2,4), (2,1), (1,5), (5,8), (8,7), (7,1),
+                     (7,2), (7,4), (4,3), (3,4), (3,3), (9, 8), (8, 1), (4,5), (5,10)]"
+
+definition "vertices = remdups (map prod.fst edges @ map prod.snd edges)"
+
+definition "c_list = [((0::nat, 1::nat), 1::real), ((0, 2), 0.5), ((2, 3), 5/8), ((2,4), 3), ((2,1), -1/3),
+                      ((1,5), 4), ((5,8), 2), ((8,7), 0.1), ((7,1), 1.3),
+                     ((7,2), 3), ((7,4), 3), ((4,3), 2), ((3,4), 1), ((3,3), 0), ((9, 8),2.5),
+                      ((8, 1), 0), ((4,5), 2), ((5,10), 3)]"
+
+definition "c_impl = foldr (\<lambda> xy tree. update (prod.fst xy) (prod.snd xy) tree) c_list Leaf"
+value "c_impl"
+
+definition "costs x y=  (case (connection_lookup c_impl (x, y)) of Some c => c | None => PInfty)"
+
+value edges
+value vertices
+
+text \<open>Select a source\<close>
+definition "init = bellman_ford_init_algo vertices 0"
+
+text \<open>Execute the Bellman-Ford loop for $n - 1$ where $n$ is the number of vertices.\<close>
+definition "final = bellman_ford_algo costs edges (length vertices - 1) init"
+value "inorder final"
+
+text \<open>Recover cheapest path from $0$ to $1$ etc.\<close>
+value "(search_rev_path_exec 0 final 1 Nil)"
+
+value "(search_rev_path_exec 0 final 10 Nil)"
+
+value "(search_rev_path_exec 0 final 4 Nil)"
+
+end
