Set_Graphs/Graph_Algorithms/DFS_Example.thy
@@ -1,0 +1,88 @@
+theory DFS_Example
+  imports DFS "HOL-Data_Structures.RBT_Map" Set2_Join_RBT
+begin
+
+definition "t_set \<equiv> Tree2.set_tree"
+definition "neighb_inv \<equiv>  (\<lambda>t. (invc t \<and> invh t) \<and> Tree2.bst t)"
+definition "neighb_empty = Leaf"
+
+notation neighb_empty ("\<emptyset>\<^sub>N")
+
+fun sel where
+"sel Leaf = undefined" |
+"sel (B l a r) = a"|
+"sel (R l a r) = a"
+
+lemma Set_satisified: "Set neighb_empty neighb_insert neighb_delete isin t_set neighb_inv"
+  using  RBT.Set_axioms 
+  by(auto simp add: neighb_empty_def neighb_delete_def neighb_insert_def t_set_def neighb_inv_def)
+
+lemma Set_Choose_axioms: "Set_Choose_axioms neighb_empty isin sel"
+  apply(rule Set_Choose_axioms.intro)
+  unfolding neighb_empty_def 
+  subgoal for s
+    by(induction rule: sel.induct) auto
+  done
+ 
+lemma Set_Choose_satisfied:"Set_Choose neighb_empty neighb_insert neighb_delete isin neighb_inv t_set sel"
+  using Set_satisified Set_Choose_axioms
+  by(auto simp add: Set_Choose_def)
+
+notation empty ("\<emptyset>\<^sub>G")
+
+lemma Map_satisfied: "Map neighb_empty update RBT_Map.delete lookup M.invar"
+  using RBT_Map.M.Map_axioms
+  by(auto simp add: Map_def M.invar_def neighb_empty_def  RBT_Set.empty_def )
+
+lemma Pair_Graph_Specs_satisfied: "Pair_Graph_Specs empty RBT_Map.delete lookup neighb_insert isin t_set sel
+     update M.invar neighb_empty neighb_delete neighb_inv"
+  using Set_Choose_satisfied Map_satisfied
+  unfolding Pair_Graph_Specs_def
+  by(auto simp add: Pair_Graph_Specs_def empty_def  neighb_empty_def)
+
+lemma Set2_satisfied: "Set2 neighb_empty neighb_delete isin t_set neighb_inv neighb_insert neighb_union
+     neighb_inter neighb_diff"
+  using  Set2_Join_RBT.RBT.Set2_axioms 
+  by(auto simp add: RBT_Set.empty_def neighb_empty_def neighb_delete_def t_set_def neighb_inv_def neighb_insert_def
+                    neighb_union_def neighb_inter_def neighb_diff_def)
+
+global_interpretation dfs: DFS 
+where insert = neighb_insert 
+and sel = sel 
+and neighb_empty = neighb_empty 
+and diff = neighb_diff 
+and lookup = lookup 
+and empty = empty 
+and delete=delete 
+and isin = isin 
+and t_set=t_set
+and update=update 
+and adj_inv = M.invar
+and neighb_delete= neighb_delete
+and neighb_inv = neighb_inv 
+and union=neighb_union 
+and inter=neighb_inter 
+and G = F and t = "t::nat" and s = "s::nat"  for F t s
+defines  dfs_initial_state = dfs.initial_state 
+and neighbourhood=dfs.Graph.neighbourhood 
+and dfs_impl = dfs.DFS_impl
+  using Pair_Graph_Specs_satisfied Set2_satisfied 
+  by(auto intro!: DFS.intro)
+
+definition "edges = [(0::nat, 1::nat), (0, 2), (2, 3), (2,4), (2,1), (1,5), (5,8), (8,7), (7,1),
+                     (7,2), (7,4), (4,3), (3,4), (3,3), (9, 8), (8, 1), (4,5), (5,10)]"
+
+definition "vertices = remdups (map prod.fst edges @ map prod.snd edges)"
+
+definition "nbs v = foldr (\<lambda> x tree. insert x tree) (remdups (map prod.snd (filter (\<lambda> e. prod.fst e = v) edges))) neighb_empty"
+
+definition "G = foldr (\<lambda> x tree. update x (nbs x) tree) vertices  empty"
+
+value edges
+value vertices
+value "neighb_diff (nbs 1) (nbs 2)"
+value G
+value "dfs_initial_state 1"   
+value "dfs_impl G 9 (dfs_initial_state 0)"
+value "dfs_impl G 3 (dfs_initial_state 0)"
+end
